Remove admits from case study

io/case-studies/Shared.fst
@@ -1,6 +1,7 @@
 module Shared
 
 open FStar.Tactics
+open FStar.Classical.Sugar
 
 open Common
 open IO.Sig
@@ -30,16 +31,16 @@ let rec is_open (fd:file_descr) (h: trace) : Tot bool =
 
 let ctx_pre (fd:file_descr) (h:trace) : Type0 = True
 
+let rec did_not_open_passwd (lt:trace) : bool =
+  match lt with
+  | [] -> true
+  | EOpenfile arg _ :: tl -> 
+      let (fnm, _, _) : io_args Openfile = arg in 
+      not (fnm = "/etc/passwd/") || did_not_open_passwd tl
+  | _ :: tl -> did_not_open_passwd tl
 
-(** The post-condition is too storng to be able to write a monitorable prop (pi).
-   The problem is that we can not prevent with the pi the closing of a file_descr by the 
-   plugin **)
-let ctx_post : file_descr -> trace -> r:(maybe unit) -> trace -> Tot (b:bool{r == Inr Contract_failure ==> b == true}) = 
-  fun fd h r lt -> 
-    match r with
-    | Inr Contract_failure -> true
-    | _ -> not (is_open fd h) || is_open fd (apply_changes h lt)
-
+let ctx_post : file_descr -> trace -> r:(maybe unit) -> trace -> Type0 = 
+  fun fd h r lt -> did_not_open_passwd lt
 
 val pi : monitorable_prop
 let pi cmd arg h =
@@ -48,18 +49,34 @@ let pi cmd arg h =
     let (fnm, _, _) : io_args Openfile = arg in not (fnm = "/etc/passwd")
   | _ -> true
 
+let rec lemma_pi_implies_did_not_open_passwd (h lt:trace) :
+  Lemma
+    (requires (enforced_locally pi h lt))
+    (ensures (did_not_open_passwd lt)) 
+    (decreases lt) =
+  match lt with
+  | [] -> ()
+  | e :: tl -> lemma_pi_implies_did_not_open_passwd (apply_changes h [e]) tl
+
 private
 let lemma_c1post_0 fd h lt :
   Lemma
     (requires (ctx_pre fd h /\ enforced_locally pi h lt))
-    (ensures (exists r. ctx_post fd h r lt)) = admit ()
+    (ensures (exists r. ctx_post fd h r lt)) = 
+  introduce exists r. ctx_post fd h r lt with (Inl ()) and begin
+    lemma_pi_implies_did_not_open_passwd h lt
+  end
 
 private
 let lemma_c1post () : squash (forall x h lt. ctx_pre x h /\ enforced_locally pi h lt ==> (exists r. ctx_post x h r lt)) = 
   Classical.forall_intro_3 (Classical.move_requires_3 (lemma_c1post_0))
 
 private
-let lemma_c2post () : squash (forall x h r lt. ctx_pre x h /\ enforced_locally pi h lt  ==> ctx_post x h r lt) = admit ()
+let lemma_c2post () : squash (forall x h r lt. ctx_pre x h /\ enforced_locally pi h lt  ==> ctx_post x h r lt) =
+  lemma_c1post ()
+
+private
+let lemma_piprop () : squash (forall h cmd arg. pi cmd arg h ==> io_pre cmd arg h) = ()
 
 instance ctx_post_monitorable () : monitorable_post ctx_pre (fun x h r lt -> ctx_post x h r lt) pi = {
   result_check = (fun _ _ _ _ -> true);
@@ -74,7 +91,7 @@ noeq type shared_interface = {
   pi : monitorable_prop;
   piprop : squash (forall h cmd arg. pi cmd arg h ==> io_pre cmd arg h);
   pre : ctx_arg -> trace -> Type0;
-  post : ctx_arg -> trace -> r:(maybe ctx_ret) -> trace -> b:Type0{r == Inr Contract_failure ==> b};
+  post : ctx_arg -> trace -> r:(maybe ctx_ret) -> trace -> Type0;
   post_c : monitorable_post pre post pi;
 }
 
@@ -83,7 +100,7 @@ let shr : shared_interface = {
   ctx_ret = unit;
   ret = unit;
   pi = pi;
-  piprop = admit ();
+  piprop = lemma_piprop ();
   pre = ctx_pre;
   post = (fun fd h r lt -> ctx_post fd h r lt);
   post_c = ctx_post_monitorable ()
