io/TC.Monitorable.Hist.fst
@@ -3,6 +3,7 @@ module TC.Monitorable.Hist
 open FStar.Tactics
 open FStar.Tactics.Typeclasses
 
+open Common
 open IO.Sig 
 
 (** why do I need action_type **)
@@ -26,13 +27,16 @@ let rec enforced_locally
     if has_event_respected_pi e check h then enforced_locally (check) (e::h) t
     else false
 
-class monitorable_post (#t1:Type) (#t2:Type) 
+class monitorable_post
+  (#t1:Type)
+  (#t2:Type) 
   (pre : t1 -> trace -> Type0)
-  (post : t1 -> trace -> t2 -> trace -> Type0)
+  (post : t1 -> trace -> maybe t2 -> trace -> Type0)
   (pi : monitorable_prop) = {
-  result_check : t1 -> trace -> t2 -> trace -> bool;
-  (** this condition makes sure that all trace properties enforced by post are instrumented by pi **)
-  c1post : squash (forall x h lt. pre x h /\ enforced_locally pi h lt ==> (exists r. post x h r lt));
-  (** this one makes sure that the post at the end is enough **)
-  c2post: squash (forall x h r lt. pre x h /\ enforced_locally pi h lt /\ result_check x h r lt ==> post x h r lt)
+    (** the refinement makes sure that the post can not reject the halting of the execution by the insturmentation **)
+    result_check : t1 -> trace -> r:maybe t2 -> trace -> (b:bool{r == Inr Contract_failure ==> b});
+    (** this condition makes sure that all trace properties enforced by post are instrumented by pi **)
+    c1post : squash (forall x h lt. pre x h /\ enforced_locally pi h lt ==> (exists r. post x h r lt));
+    (** this one makes sure that the post at the end is enough **)
+    c2post: squash (forall x h r lt. pre x h /\ enforced_locally pi h lt /\ result_check x h r lt ==> post x h r lt);
 }
